update

theory/Sound_Communication_A.thy
@@ -1221,7 +1221,7 @@ inductive narrow_step :: "trace_pool * cmmn_set \<Rightarrow> control_path \<Rig
   step: "
     concur_step (E, H) (Em, Hm) \<Longrightarrow>
     leaf E \<pi> \<Longrightarrow>
-    Em (\<pi> @ [l]) \<noteq> None \<Longrightarrow>
+    leaf Em (\<pi> @ [l]) \<Longrightarrow>
     narrow_step (Em, Hm) (\<pi> @ [l]) (E', H') \<pi>' \<Longrightarrow>
     narrow_step (E, H) \<pi> (E', H') \<pi>'
   "
@@ -1243,6 +1243,106 @@ lemma static_traversable_pool_implies_static_traceabl_generalized:
       static_traceable V F (top_label e) isEnd path"
 
 sorry
+
+lemma step_in_line: 
+  assumes 
+    H1: "concur_step (E, H) (Em, Hm)" and
+    H2: "star concur_step (Em, Hm) (E', H')" and
+    H3: "leaf E \<pi>" and
+    H4: "E' \<pi>' \<noteq> None" and
+    H5: "strict_prefix \<pi> \<pi>'"
+
+  shows "\<exists> l . leaf Em (\<pi> @ [l]) \<and> prefix (\<pi> @ [l]) \<pi>'"
+proof -
+  
+  obtain EH EHm EH' where
+    H6: "EH = (E, H)" and H7: "EHm = (Em, Hm)" and H8: "EH' = (E', H')"
+    by simp
+
+  have H9: "star concur_step EHm EH'"
+    by (simp add: H2 H7 H8)
+
+  have H10: "
+    \<forall> E H \<pi> Em Hm .
+    EH = (E, H) \<longrightarrow> EHm = (Em, Hm) \<longrightarrow> EH' = (E', H') \<longrightarrow>
+    concur_step (E, H) (Em, Hm) \<longrightarrow>
+    leaf E \<pi> \<longrightarrow> strict_prefix \<pi> \<pi>' \<longrightarrow>
+    (\<exists> l . leaf Em (\<pi> @ [l]) \<and> prefix (\<pi> @ [l]) \<pi>')
+  "
+  using H9
+  proof induction
+    case (refl x)
+    {
+      fix E H \<pi> Em Hm
+      assume
+        L2H1: "EH = (E, H)" and
+        L2H2: "x = (Em, Hm)" and
+        L2H3: "x = (E', H')" and 
+        L2H4: "(E, H) \<rightarrow> (Em, Hm)" and
+        L2H5: "leaf E \<pi>" and
+        L2H6: "strict_prefix \<pi> \<pi>'"
+
+      have L2H7: "Em = E'" using L2H2 L2H3 by auto
+
+
+      have L2H8: "E \<pi>' = None" using L2H5 L2H6 using leaf.cases by auto
+
+      have L2H9: "(E, H) \<rightarrow> (E', H')"  using L2H2 L2H3 L2H4 by blast
+
+      have L2H10: "\<exists>l. leaf E' (\<pi> @ [l]) \<and> prefix (\<pi> @ [l]) \<pi>'"
+      using L2H9
+      proof cases
+        case (Seq_Step_Down pi x env xk ek envk k v)
+        then show ?thesis
+          by (smt H4 L2H5 L2H6 fun_upd_other leaf.simps prefix_order.le_less_trans prefix_snoc strict_prefix_def)
+      next
+        case (Seq_Step pi x b e env k v)
+        then show ?thesis
+          by (smt H4 L2H5 L2H6 fun_upd_other leaf.simps prefix_order.le_less_trans prefix_snoc strict_prefix_def)
+      next
+        case (Seq_Step_Up pi x b e env k e' env')
+        then show ?thesis
+          by (smt H4 L2H5 L2H6 fun_upd_other leaf.simps prefix_order.le_less_trans prefix_snoc strict_prefix_def)
+      next
+        case (Let_Chan pi x e env k)
+        then show ?thesis 
+          by (smt H4 L2H5 L2H6 fun_upd_other leaf.simps prefix_order.le_less_trans prefix_snoc strict_prefix_def)
+      next
+        case (Let_Spawn pi x ec e env k)
+        then show ?thesis
+          by (smt H4 L2H5 L2H6 fun_upd_other leaf.simps prefix_order.le_less_trans prefix_snoc strict_prefix_def)
+      next
+        case (Let_Sync pis xs xse es envs ks xsc xm envse pir xr xre er envr kr xrc envre c vm)
+        then show ?thesis
+          by (smt H4 L2H5 L2H6 fun_upd_other leaf.simps prefix_order.le_less_trans prefix_snoc strict_prefix_def)
+      qed
+
+      have "\<exists>l. leaf Em (\<pi> @ [l]) \<and> prefix (\<pi> @ [l]) \<pi>'"
+        by (simp add: L2H7 L2H10)
+    }
+    then show ?case by blast
+  next
+    case (step x y z)    
+    {
+      fix E H \<pi> Em Hm
+      assume
+        L2H1: "EH = (E, H)" and
+        L2H2: "x = (Em, Hm)" and
+        L2H3: "z = (E', H')" and 
+        L2H4: "(E, H) \<rightarrow> (Em, Hm)" and
+        L2H5: "leaf E \<pi>" and
+        L2H6: "strict_prefix \<pi> \<pi>'"
+
+      have "\<exists>l. leaf Em (\<pi> @ [l]) \<and> prefix (\<pi> @ [l]) \<pi>'" sorry
+    }
+
+    then show ?case by blast
+  qed
+
+  show ?thesis 
+    by (simp add: H1 H10 H3 H5 H6 H7 H8)
+qed
+
 
 lemma star_concur_step_implies_narrow_step: 
   assumes 
@@ -1290,49 +1390,24 @@ proof -
         L2H4: "E' \<pi>' \<noteq> None" and 
         L2H5: "prefix \<pi> \<pi>'"
 
-
-      have
-        L2H9: "\<exists> l Em Hm . y = (Em, Hm) \<and> leaf Em (\<pi> @ [l]) \<and> prefix (\<pi> @ [l]) \<pi>'"
-      using step.hyps(1)
-      proof cases
-        case (Seq_Step_Down pi x env xk ek envk k v)
-        then show ?thesis sorry
-      next
-        case (Seq_Step pi x b e env k v)
-        then show ?thesis sorry
-      next
-        case (Seq_Step_Up pi x b e env k e' env')
-        then show ?thesis sorry
-      next
-        case (Let_Chan pi x e env k)
-        then show ?thesis sorry
-      next
-        case (Let_Spawn pi x ec e env k)
-        then show ?thesis sorry
-      next
-        case (Let_Sync pis xs xse es envs ks xsc xm envse pir xr xre er envr kr xrc envre c vm)
-        then show ?thesis sorry
-      qed
-
-
-
     
-      obtain Em Hm l where L2H10: "y = (Em, Hm) \<and> leaf Em (\<pi> @ [l]) \<and> prefix (\<pi> @ [l]) \<pi>'" using L2H9 by blast
+      obtain Em Hm where 
+        L2H6: "y = (Em, Hm)" by fastforce
+    
+      obtain l where
+        L2H7: "leaf Em (\<pi> @ [l])" and
+        L2H8: "prefix (\<pi> @ [l]) \<pi>'"
+        using L2H1 L2H2 L2H3 L2H4 L2H5 L2H6 step.hyps(1) step.hyps(2) step_in_line by blast
+    
+      have L2H9: "narrow_step (Em, Hm) (\<pi> @ [l]) (E', H') \<pi>'"
+        using L2H2 L2H4 L2H6 L2H7 L2H8 step.hyps(3) by blast
 
-      have "L2H11": "narrow_step (Em, Hm) (\<pi> @ [l]) (E', H') \<pi>'"
-        using L2H10 L2H2 L2H4 L2H9 step.hyps(3) by blast
-
-      have L2H12: "Em (\<pi> @ [l]) \<noteq> None" using leaf.simps L2H10 by blast
-
-      have L2H13: "narrow_step (E, H) \<pi> (E', H') \<pi>'"
-        using L2H1 L2H11 L2H12 L2H3 L2H10 narrow_step.step step.hyps(1) by blast
-
-      have "narrow_step x \<pi> z \<pi>'" by (simp add: L2H1 L2H13 L2H2)
+      have "narrow_step x \<pi> z \<pi>'" using narrow_step.step
+        using L2H1 L2H2 L2H3 L2H6 L2H7 L2H8 L2H9 step.hyps(1) by blast
+ 
     }
-
     then show ?case by blast
   qed
-
   show ?thesis using H2 H3 H4 H5 H6 by blast
 qed
 
